Examples/RingDSL.lean
@@ -1,0 +1,108 @@
+import LeanSts.State
+import LeanSts.TransitionSystem
+import LeanSts.Tactics
+-- import Mathlib.Tactic
+import LeanSts.DSL
+
+-- https://github.com/aman-goel/ivybench/blob/5db7eccb5c3bc2dd14dfb58eddb859b036d699f5/ex/ivy/ring.ivy
+
+section RingPrec
+
+
+class TotalOrder (t : Type) :=
+  -- relation: total order
+  le (x y : t) : Bool
+  -- axioms
+  le_refl       (x : t) : le x x
+  le_trans  (x y z : t) : le x y → le y z → le x z
+  le_antisymm (x y : t) : le x y → le y x → x = y
+  le_total    (x y : t) : le x y ∨ le y x
+
+class Between (node : Type) :=
+  -- relation: btw represents a ring
+  -- read: y is between x and z
+  btw (x y z : node) : Bool
+  -- axioms
+  btw_ring    (x y z : node) : btw x y z → btw y z x
+  btw_trans (w x y z : node) : btw w x y → btw w y z → btw w x z
+  btw_side    (w x y : node) : btw w x y → ¬ btw w y x
+  btw_total   (w x y : node) : btw w x y ∨ btw w y x ∨ w = x ∨ w = y ∨ x = y
+
+variable (node : Type)
+variable [DecidableEq node] [TotalOrder node] [Between node]
+
+open Between TotalOrder
+
+theorem btw_irreflexive : ∀ (n m : node),  ¬ btw m n n := by
+  duper [btw_side] {portfolioInstance := 1}
+
+theorem btw_irreflexive' : ∀ (n m : node), ¬ btw m m n := by
+  duper [btw_ring, btw_side] {portfolioInstance := 1}
+
+theorem btw_arg : ∀ (a b c : node), btw a b c →
+  ¬ a = b ∧ ¬ a = c ∧ ¬ b = c := by
+  duper [btw_ring, btw_trans, btw_side, Between.btw_total] {portfolioInstance := 1}
+
+theorem btw_next :
+  (∀ (z : node), n ≠ next ∧ ((z ≠ n ∧ z ≠ next) → btw n next z)) →
+  (∀ (z : node), ¬ btw n z next) := by
+  duper [btw_ring, btw_trans, btw_side, Between.btw_total] {portfolioInstance := 1}
+
+theorem btw_opposite
+  (Hn : ∀ (z : node), ¬ btw n z next = true)
+  (h1 : btw sender N next = true)
+  (h2 : btw sender n N = true) :
+  False := by
+  duper [Hn, h1, h2, btw_ring, btw_trans] {portfolioInstance := 1}
+
+end RingPrec
+
+section Ring
+open Between TotalOrder
+
+type node
+instantiate DecidableEq node
+instantiate TotalOrder node
+instantiate Between node
+
+relation leader : node -> Bool
+relation pending : node -> node -> Bool
+
+#gen_state
+
+#print State
+
+initial = fun rs =>
+  (∀ (n : node), ¬ rs.leader n) ∧
+  (∀ (n1 n2 : node), ¬ rs.pending n1 n2)
+
+action send (n next : node) :=
+   λ (st st' : State node) =>
+      -- preconditions
+      (∀ (z : node), n ≠ next ∧ ((z ≠ n ∧ z ≠ next) → Between.btw n next z)) ∧
+      -- postconditions
+      st' = {st with pending := st.pending[n , next ↦ true]}
+
+
+action recv (sender n next : node) (havoc : Bool) :=
+  λ (st st' : State node) =>
+      -- preconditions
+      (∀ (z : node), n ≠ next ∧ ((z ≠ n ∧ z ≠ next) → Between.btw n next z)) ∧
+      (st.pending sender n) ∧
+      -- postconditions
+      -- `pending(sender, n) := *` is modelled using `havoc`
+      if sender = n then
+        st' = {st with leader := st.leader[n ↦ true], pending := st.pending[sender, n ↦ havoc]}
+      else
+        if TotalOrder.le n sender then
+          st' = {st with pending := st.pending[sender, n ↦ havoc][sender , next ↦ true]}
+        else
+          st' = {st with pending := st.pending[sender, n ↦ havoc]}
+
+safety = fun st => ∀ (N L : node), st.leader L → le N L
+invariant = fun st => ∀ (S D N : node), st.pending S D ∧ btw S N D → le N S
+invariant = fun st =>  ∀ (N L : node), st.pending L L → le N L
+
+#gen_spec
+
+end Ring
