LeanSts/DSLUtil.lean
@@ -17,15 +17,16 @@ def _root_.Lean.EnvExtension.modify [Inhabited σ] (ext : EnvExtension σ) (s : 
 def _root_.Lean.EnvExtension.get [Inhabited σ] (ext : EnvExtension σ) : AttrM σ := do
   return ext.getState (<- getEnv)
 
-def fresh [Monad m] [Lean.MonadLCtx m] (suggestion : Lean.Name) : m Lean.Syntax.Ident := do
-  let name ← getUnusedUserName suggestion
-  return Lean.mkIdent name
+-- def fresh [Monad m] [Lean.MonadLCtx m] (suggestion : Lean.Name) : m Lean.Syntax.Ident := do
+--   let name ← getUnusedUserName suggestion
+--   return Lean.mkIdent name
 
 structure StsState where
   typ        : Expr
   rel_sig    : Array (TSyntax `Lean.Parser.Command.structSimpleBinder)
   init       : Expr
   actions    : List Expr
+  safety     : Expr
   invariants : List Expr
   deriving Inhabited
 
@@ -34,7 +35,7 @@ open StsState
 initialize stsExt : EnvExtension StsState ←
   registerEnvExtension (pure default)
 
-syntax (name:= state) "state" : attr
+syntax (name:= state) "stateDef" : attr
 
 initialize registerBuiltinAttribute {
   name := `state
@@ -47,7 +48,7 @@ initialize registerBuiltinAttribute {
     stsExt.modify ({ · with typ := ty })
 }
 
-syntax (name:= initial) "initial" : attr
+syntax (name:= initial) "initDef" : attr
 
 initialize registerBuiltinAttribute {
   name := `initial
@@ -56,12 +57,12 @@ initialize registerBuiltinAttribute {
     -- Check if the initial state has already been declared
     let intTp := (<- stsExt.get).init
     unless intTp == default do
-      throwError "Inital state predicate has already been declared: {intTp}"
+      throwError "Inital state predicate has already been declared"
     let init := mkConst declName
     stsExt.modify ({ · with init := init })
 }
 
-syntax (name:= action) "action" : attr
+syntax (name:= action) "actDef" : attr
 
 initialize registerBuiltinAttribute {
   name := `action
@@ -70,7 +71,21 @@ initialize registerBuiltinAttribute {
     stsExt.modify (fun s => { s with actions := mkConst declName :: s.actions})
 }
 
-syntax (name:= inv) "inv" : attr
+syntax (name:= safe) "safeDef" : attr
+
+initialize registerBuiltinAttribute {
+  name := `safe
+  descr := "Marks as a safety property"
+  add := fun declName _ _ => do
+    -- Check if the initial state has already been declared
+    let safety := (<- stsExt.get).safety
+    unless safety == default do
+      throwError "Safety predicate has already been declared"
+    stsExt.modify ({ · with safety := mkConst declName })
+}
+
+
+syntax (name:= inv) "invDef" : attr
 
 initialize registerBuiltinAttribute {
   name := `inv
@@ -78,3 +93,8 @@ initialize registerBuiltinAttribute {
   add := fun declName _ _ => do
     stsExt.modify (fun s => { s with invariants := mkConst declName :: s.invariants})
 }
+
+register_simp_attr invSimp
+register_simp_attr actSimp
+register_simp_attr initSimp
+register_simp_attr safeSimp
