LeanSts/TransitionSystem.lean
@@ -25,16 +25,19 @@ class RelationalTransitionSystem (σ : Type) extends
   where
   init : σ → Prop
   next : RelationalTransitionSystem.action σ
-  -- safety : σ → Prop
+  safe : σ → Prop
   inv : σ → Prop
 
 open RelationalTransitionSystem
 
-def inv_init [RelationalTransitionSystem σ] :=
+def invInit [RelationalTransitionSystem σ] :=
   ∀ (s : σ), init s -> inv s
 
-def inv_inductive [RelationalTransitionSystem σ] :=
-  ∀ (s1 s2 : σ), next s1 s2 -> inv s1 -> inv s2
+def safetyInit [RelationalTransitionSystem σ] :=
+  ∀ (s : σ), init s -> safe s
+
+def invInductive [RelationalTransitionSystem σ] :=
+  ∀ (s1 s2 : σ), next s1 s2 -> safe s1 ∧ inv s1 -> safe s2 ∧ inv s2
 
 
 class FunctionalTransitionSystem (σ : Type) extends
